code/jasmin/mlkem_avx2_stack/extraction/WArray33.ec
@@ -1,0 +1,3 @@
+from Jasmin require import JWord_array.
+
+clone export WArray as WArray33  with op size <- 33.
