proof/correctness/avx2/MLKEM_KEM_avx2_stack.ec
@@ -1,0 +1,51 @@
+require import AllCore IntDiv List.
+require import Jkem_avx2_stack MLKEM.
+from Jasmin require import JModel_x86.
+
+require import Array32 Array64 Array960 Array128 Array1088 Array1152 Array1184 Array2400.
+import MLKEM.
+
+print MLKEM.
+
+lemma mlkem_kem_correct_kg   : 
+   equiv [Jkem_avx2_stack.M.jade_kem_mlkem_mlkem768_amd64_avx2_keypair_derand ~ MLKEM.kg_derand : 
+        coins{2}.`1 = Array32.init(fun i => coins{1}.[i]) /\
+        coins{2}.`2 = Array32.init(fun i => coins{1}.[32 + i]) 
+        ==> 
+       let (pk,sk) = res{2} in let (t,rho) = pk in
+         sk.`1 = Array1152.init(fun i => res{1}.`1.[i])  /\
+         sk.`2.`1 = Array1152.init(fun i => res{1}.`1.[i+1152]) /\
+         sk.`2.`2 = Array32.init(fun i => res{1}.`1.[i+1152+1152]) /\
+         sk.`3 = Array32.init(fun i => res{1}.`1.[i+1152+1152 + 32]) /\
+         sk.`4 = Array32.init(fun i => res{1}.`1.[i+1152+1152 + 32 + 32]) /\
+         t = Array1152.init(fun i => res{1}.`2.[i]) /\  
+         rho = Array32.init(fun i => res{1}.`2.[i+1152])].
+admitted.
+
+lemma mlkem_kem_correct_enc : 
+   equiv [Jkem_avx2_stack.M.jade_kem_mlkem_mlkem768_amd64_avx2_enc_derand ~ MLKEM.enc_derand: 
+     coins{1} = coins{2} /\
+     pk{2}.`1 = Array1152.init(fun i => public_key{1}.[i])  /\
+     pk{2}.`2 = Array32.init(fun i => public_key{1}.[i+1152])
+       ==> 
+     let (c,k) = res{2} in
+     c.`1 = Array960.init(fun i => res{1}.`1.[i]) /\
+     c.`2 = Array128.init(fun i => res{1}.`1.[i+960])  /\
+     k = res{1}.`2
+].
+admitted.
+
+lemma mlkem_kem_correct_dec : 
+   equiv [Jkem_avx2_stack.M.jade_kem_mlkem_mlkem768_amd64_avx2_dec ~ MLKEM.dec: 
+      sk{2}.`1 = Array1152.init(fun i => secret_key{1}.[i])  /\
+      sk{2}.`2.`1 = Array1152.init(fun i => secret_key{1}.[i+1152]) /\
+      sk{2}.`2.`2 = Array32.init(fun i => secret_key{1}.[i+1152+1152]) /\
+      sk{2}.`3 = Array32.init(fun i => secret_key{1}.[i+1152+1152 + 32]) /\
+      sk{2}.`4 = Array32.init(fun i => secret_key{1}.[i+1152+1152 + 32 + 32]) /\
+     let (c1,c2) = cph{2} in
+         cph{2}.`1 = Array960.init(fun i => ciphertext{1}.[i]) /\
+         cph{2}.`2 = Array128.init(fun i => ciphertext{1}.[i+960])  
+       ==> 
+     res{2} = res{1}.`1
+].
+admitted.
